src/Value.v
@@ -15,6 +15,31 @@ Context `{HostExprs A}.
 
 Open Scope Ty_scope.
 
+(* [ValueP] is an inductive proposition that indicates whether an expression
+   represents a value, i.e., that it does reduce any further. *)
+Inductive ValueP Γ : ∀ {τ}, Exp Γ τ → Type :=
+  | HostedValP {ty} (x : HostExp (TyHost ty)) : ValueP Γ (HostedVal x)
+  | HostedFunP {dom cod} (f : HostExp (dom ⟶ cod)) : ValueP Γ (HostedFun f)
+  | UnitP : ValueP Γ EUnit
+  | TrueP : ValueP Γ ETrue
+  | FalseP : ValueP Γ EFalse
+  | PairP {τ1 τ2} {x : Exp Γ τ1} {y : Exp Γ τ2} :
+    ValueP Γ x → ValueP Γ y → ValueP Γ (Pair x y)
+  | NilP {τ} : ValueP Γ (Nil (τ:=τ))
+  | ConsP {τ} (x : Exp Γ τ) xs :
+    ValueP Γ x → ValueP Γ xs → ValueP Γ (Cons x xs)
+  | LambdaP {dom cod} (e : Exp (dom :: Γ) cod) : ValueP Γ (LAM e).
+
+Derive Signature NoConfusion NoConfusionHom for ValueP.
+
+Lemma ValueP_irrelevance {Γ τ} (v : Exp Γ τ) (H1 H2 : ValueP _ v) :
+  H1 = H2.
+Proof.
+  induction H1; dependent elimination H2; auto.
+  - now erewrite IHValueP1, IHValueP2; eauto.
+  - now erewrite IHValueP1, IHValueP2; eauto.
+Qed.
+
 Inductive Value : Ty → Type :=
   | HostValue {ty}         : HostExp (TyHost ty) → Value (TyHost ty)
   | VUnit                  : Value TyUnit
@@ -43,3 +68,13 @@ Equations get_value `(s : ValEnv Γ) `(v : Var Γ τ) : Value τ :=
   get_value (Val _ xs) (SV v) := get_value xs v.
 
 End Value.
+
+Arguments ValueP {A H Γ τ} _.
+Arguments HostedValP {A H Γ ty} _.
+Arguments HostedFunP {A H Γ dom cod} _.
+Arguments TrueP {A H Γ}.
+Arguments FalseP {A H Γ}.
+Arguments PairP {A H Γ τ1 τ2 x y} _ _.
+Arguments NilP {A H Γ τ}.
+Arguments ConsP {A H Γ τ _ _} _ _.
+Arguments LambdaP {A H Γ dom cod} _.
