src/Ltac.v
@@ -13,9 +13,19 @@ Ltac reduce_jmeq :=
       specialize (H _ JMeq_refl JMeq_refl JMeq_refl)
   | [ H : ∀ _: _, _ ~= _ → _ ~= _ → _ ~= _ → _ ~= _ → _ |- _ ] =>
       specialize (H _ JMeq_refl JMeq_refl JMeq_refl JMeq_refl)
+
+  | [ H : ∀ _ _ _, _ = _ → _ ~= _ → _ |- _ ] =>
+      specialize (H _ _ _ eq_refl JMeq_refl)
+  | [ H : ∀ _ _ _, _ = _ → _ ~= _ → _ ~= _ → _ |- _ ] =>
+      specialize (H _ _ _ eq_refl JMeq_refl JMeq_refl)
+  | [ H : ∀ _ _ _, _ = _ → _ ~= _ → _ ~= _ → _ ~= _ → _ |- _ ] =>
+      specialize (H _ _ _ eq_refl JMeq_refl JMeq_refl JMeq_refl)
+  | [ H : ∀ _ _ _, _ = _ → _ ~= _ → _ ~= _ → _ ~= _ → _ ~= _ → _ |- _ ] =>
+      specialize (H _ _ _ eq_refl JMeq_refl JMeq_refl JMeq_refl JMeq_refl)
   end.
 
 Ltac reduce :=
+  reduce_jmeq;
   repeat (match goal with
           | [ H : existT _ _ _ = existT _ _ _ |- _ ] =>
               apply inj_pair2 in H; subst
@@ -24,6 +34,6 @@ Ltac reduce :=
           | [ H : ∃ _, _ |- _ ] => destruct H
           | [ H : { _ : _ | _ } |- _ ] => destruct H
           | [ H : { _ : _ & _ } |- _ ] => destruct H
-          end; reduce_jmeq; subst).
+          end; subst).
 
 Ltac inv H := inversion H; subst; clear H; reduce.
