src/Sem.v
@@ -108,6 +108,8 @@ Fixpoint SemExp `(e : Exp Γ τ) : SemEnv Γ → SemTy τ :=
   | Snd p         => λ se, snd (SemExp p se)
   | Nil           => λ se, nil
   | Cons x xs     => λ se, SemExp x se :: SemExp xs se
+  | Car d xs      => λ se, hd (SemExp d se) (SemExp xs se)
+  | Cdr xs        => λ se, tl (SemExp xs se)
   | Seq exp1 exp2 => λ se, SemExp exp2 se
 
   | VAR v         => SemVar v
@@ -146,6 +148,8 @@ Proof.
   - now rewrite IHe.
   - now rewrite IHe.
   - now rewrite IHe1, IHe2.
+  - now rewrite IHe1, IHe2.
+  - now rewrite IHe.
   - now rewrite SemVar_RenSem.
   - extensionality z.
     fold SemTy in z.
@@ -218,6 +222,8 @@ Proof.
   - now rewrite IHe.
   - now rewrite IHe.
   - now rewrite IHe1, IHe2.
+  - now rewrite IHe1, IHe2.
+  - now rewrite IHe.
   - now rewrite SemVar_SubSem.
   - extensionality z.
     fold SemTy in z.
